Improved presentation

BDD.thy
@@ -1,20 +1,19 @@
 
 theory BDD
   imports
-    Bij_betw_simplicial_complex_bool_func
+    Evasive
     ROBDD.Level_Collapse
     ListLexorder
 begin
 
-section\<open>Relation between boolean functions over vectors and boolfunc as in ROBDD\<close>
-
-definition vec_to_boolfunc :: "nat => (bool vec => bool) => nat boolfunc"
-  where "vec_to_boolfunc n f = (\<lambda>p. f (vec n p))"
-
-text \<open>Each vertex in a simplicial complex corresponds to one True line in the truth table of the inducing boolean function.\<close>
+text \<open>Each vertex in a simplicial complex corresponds to one @{term True} line 
+  in the truth table of the inducing Boolean function.\<close>
 
 definition bf_from_sc :: "nat set set => (bool vec \<Rightarrow> bool)" 
-  where "bf_from_sc K \<equiv> (\<lambda>v. {i. i < dim_vec v \<and> vec_index v i = False} \<in> K)"
+  where "bf_from_sc K \<equiv> (\<lambda>v. {i. i < dim_vec v \<and> \<not> (vec_index v i)} \<in> K)"
+
+(*definition bf_from_sc :: "nat set set => (bool vec \<Rightarrow> bool)" 
+  where "bf_from_sc K \<equiv> (\<lambda>v. {i. i < dim_vec v \<and> vec_index v i = False} \<in> K)"*)
 
 lemma bf_from_sc: 
   assumes sc: "simplicial_complex.simplicial_complex n K"
@@ -24,7 +23,8 @@ lemma bf_from_sc:
   unfolding simplicial_complex.simplicial_complex_def
   unfolding simplicial_complex.simplices_def
   unfolding ceros_of_boolean_input_def
-  by auto (metis ceros_of_boolean_input_def dim_vec sc simplicial_complex.ceros_of_boolean_input_in_set simplicial_complex.simplicial_complex_def)
+  by auto (metis ceros_of_boolean_input_def dim_vec sc 
+      simplicial_complex.ceros_of_boolean_input_in_set simplicial_complex.simplicial_complex_def)
 
 definition boolfunc_from_sc :: "nat => nat set set \<Rightarrow> nat boolfunc" 
   where "boolfunc_from_sc n K \<equiv> \<lambda>p. {i. i < n \<and> \<not> p i} \<in> K"
@@ -38,118 +38,124 @@ lemma hlp1: "{i. i < 4 \<and> \<not> (f(0 := a0, 1 := a1, 2 := a2, 3 := a3)) i} 
 \<union> (if a3 then {} else {3})" 
   by auto
 
-lemma sc_threshold_2_3_ffff: "boolfunc_from_sc 4 sc_threshold_2_3 (a (0:=False,1:=False,2:=False,3:=False)) = False"
+lemma sc_threshold_2_3_ffff: 
+  "boolfunc_from_sc 4 sc_threshold_2_3 (a (0:=False,1:=False,2:=False,3:=False)) = False"
   unfolding hlp1 boolfunc_from_sc_def sc_threshold_2_3_def
-  by simp (smt (z3) Suc_eq_numeral insert_absorb insert_commute insert_ident insert_not_empty numeral_2_eq_2 singleton_inject zero_neq_numeral)
+  by simp (smt (z3) Suc_eq_numeral insert_absorb insert_commute insert_ident 
+      insert_not_empty numeral_2_eq_2 singleton_inject zero_neq_numeral)
   
-lemma sc_threshold_2_3_ffft: "boolfunc_from_sc 4 sc_threshold_2_3 (a(0:=False,1:=False,2:=False,3:=True)) = False"
+lemma sc_threshold_2_3_ffft: 
+  "boolfunc_from_sc 4 sc_threshold_2_3 (a(0:=False,1:=False,2:=False,3:=True)) = False"
   unfolding hlp1 boolfunc_from_sc_def sc_threshold_2_3_def  
-  by simp (smt (z3) Suc_eq_numeral insertI1 insert_absorb insert_commute insert_ident insert_not_empty numeral_2_eq_2 singleton_inject zero_neq_numeral)
+  by simp (smt (z3) Suc_eq_numeral insertI1 insert_absorb insert_commute 
+      insert_ident insert_not_empty numeral_2_eq_2 singleton_inject zero_neq_numeral)
 
-lemma sc_threshold_2_3_fftf: "boolfunc_from_sc 4 sc_threshold_2_3 (a(0:=False,1:=False,2:=True,3:=False)) = False"
+lemma sc_threshold_2_3_fftf: 
+  "boolfunc_from_sc 4 sc_threshold_2_3 (a(0:=False,1:=False,2:=True,3:=False)) = False"
   unfolding hlp1 boolfunc_from_sc_def sc_threshold_2_3_def
-  by simp (smt (z3) insertI1 insert_iff numeral_1_eq_Suc_0 numeral_2_eq_2 numeral_eq_iff semiring_norm(86) singleton_iff zero_neq_numeral)
+  by simp (smt (z3) insertI1 insert_iff numeral_1_eq_Suc_0 
+      numeral_2_eq_2 numeral_eq_iff semiring_norm(86) singleton_iff zero_neq_numeral)
 
-lemma sc_threshold_2_3_ftff: "boolfunc_from_sc 4 sc_threshold_2_3 (a(0:=False,1:=True,2:=False,3:=False)) = False"
+lemma sc_threshold_2_3_ftff: 
+  "boolfunc_from_sc 4 sc_threshold_2_3 (a(0:=False,1:=True,2:=False,3:=False)) = False"
   unfolding hlp1 boolfunc_from_sc_def sc_threshold_2_3_def
-  by simp (smt (verit, ccfv_SIG) insert_absorb insert_iff insert_not_empty numeral_eq_iff semiring_norm(89) zero_neq_numeral)
+  by simp (smt (verit, ccfv_SIG) insert_absorb insert_iff insert_not_empty 
+      numeral_eq_iff semiring_norm(89) zero_neq_numeral)
  
-lemma sc_threshold_2_3_tfff: "boolfunc_from_sc 4 sc_threshold_2_3 (a(0:=True , 1:=False, 2:=False, 3:=False)) = False"
+lemma sc_threshold_2_3_tfff: 
+  "boolfunc_from_sc 4 sc_threshold_2_3 (a(0:=True,1:=False,2:=False,3:=False)) = False"
   unfolding hlp1 boolfunc_from_sc_def sc_threshold_2_3_def
-  by simp (smt (z3) eval_nat_numeral(3) insertI1 insert_commute insert_iff n_not_Suc_n numeral_1_eq_Suc_0 numeral_2_eq_2 numeral_eq_iff singletonD verit_eq_simplify(12))
+  by simp (smt (z3) eval_nat_numeral(3) insertI1 insert_commute insert_iff 
+      n_not_Suc_n numeral_1_eq_Suc_0 numeral_2_eq_2 numeral_eq_iff singletonD verit_eq_simplify(12))
 
-lemma sc_threshold_2_3_fftt: "boolfunc_from_sc 4 sc_threshold_2_3 (a(0:=False, 1:=False, 2:=True, 3:=True )) = True"
+lemma sc_threshold_2_3_fftt: 
+  "boolfunc_from_sc 4 sc_threshold_2_3 (a(0:=False,1:=False,2:=True,3:=True)) = True"
   unfolding hlp1 boolfunc_from_sc_def sc_threshold_2_3_def by auto
 
-lemma sc_threshold_2_3_ftft: "boolfunc_from_sc 4 sc_threshold_2_3 (a(0:=False, 1:=True , 2:=False, 3:=True )) = True"
+lemma sc_threshold_2_3_ftft: 
+  "boolfunc_from_sc 4 sc_threshold_2_3 (a(0:=False,1:=True,2:=False,3:=True)) = True"
   unfolding hlp1 boolfunc_from_sc_def sc_threshold_2_3_def by auto
 
-lemma sc_threshold_2_3_fttf: "boolfunc_from_sc 4 sc_threshold_2_3 (a(0:=False, 1:=True , 2:=True , 3:=False)) = True"
+lemma sc_threshold_2_3_fttf: 
+  "boolfunc_from_sc 4 sc_threshold_2_3 (a(0:=False,1:=True,2:=True,3:=False)) = True"
   unfolding hlp1 boolfunc_from_sc_def sc_threshold_2_3_def by auto
 
-lemma sc_threshold_2_3_fttt: "boolfunc_from_sc 4 sc_threshold_2_3 (a(0:=False, 1:=True , 2:=True , 3:=True )) = True"
+lemma sc_threshold_2_3_fttt: 
+  "boolfunc_from_sc 4 sc_threshold_2_3 (a(0:=False,1:=True,2:=True,3:=True)) = True"
   unfolding hlp1 boolfunc_from_sc_def sc_threshold_2_3_def by auto
 
-lemma sc_threshold_2_3_tfft: "boolfunc_from_sc 4 sc_threshold_2_3 (a(0:=True , 1:=False, 2:=False, 3:=True )) = True"
+lemma sc_threshold_2_3_tfft: 
+  "boolfunc_from_sc 4 sc_threshold_2_3 (a(0:=True,1:=False,2:=False,3:=True)) = True"
   unfolding hlp1 boolfunc_from_sc_def sc_threshold_2_3_def by auto
 
-lemma sc_threshold_2_3_tftf: "boolfunc_from_sc 4 sc_threshold_2_3 (a(0:=True , 1:=False, 2:=True , 3:=False)) = True" 
+lemma sc_threshold_2_3_tftf: 
+  "boolfunc_from_sc 4 sc_threshold_2_3 (a(0:=True,1:=False,2:=True,3:=False)) = True" 
   unfolding hlp1 boolfunc_from_sc_def sc_threshold_2_3_def by auto
 
-lemma sc_threshold_2_3_tftt: "boolfunc_from_sc 4 sc_threshold_2_3 (a(0:=True , 1:=False, 2:=True , 3:=True )) = True"
+lemma sc_threshold_2_3_tftt: 
+  "boolfunc_from_sc 4 sc_threshold_2_3 (a(0:=True,1:=False,2:=True,3:=True)) = True"
   unfolding hlp1 boolfunc_from_sc_def sc_threshold_2_3_def by auto
 
-lemma sc_threshold_2_3_ttff: "boolfunc_from_sc 4 sc_threshold_2_3 (a(0:=True , 1:=True , 2:=False, 3:=False)) = True" 
+lemma sc_threshold_2_3_ttff: 
+  "boolfunc_from_sc 4 sc_threshold_2_3 (a(0:=True,1:=True,2:=False,3:=False)) = True" 
   unfolding hlp1 boolfunc_from_sc_def sc_threshold_2_3_def by auto
 
-lemma sc_threshold_2_3_ttft: "boolfunc_from_sc 4 sc_threshold_2_3 (a(0:=True , 1:=True , 2:=False, 3:=True )) = True" 
+lemma sc_threshold_2_3_ttft: 
+  "boolfunc_from_sc 4 sc_threshold_2_3 (a(0:=True,1:=True,2:=False,3:=True)) = True" 
   unfolding hlp1 boolfunc_from_sc_def sc_threshold_2_3_def by auto
 
-lemma sc_threshold_2_3_tttf: "boolfunc_from_sc 4 sc_threshold_2_3 (a(0:=True , 1:=True , 2:=True , 3:=False)) = True "
+lemma sc_threshold_2_3_tttf: 
+  "boolfunc_from_sc 4 sc_threshold_2_3 (a(0:=True,1:=True,2:=True,3:=False)) = True "
   unfolding hlp1 boolfunc_from_sc_def sc_threshold_2_3_def by auto
 
-lemma sc_threshold_2_3_tttt: "boolfunc_from_sc 4 sc_threshold_2_3 (a(0:=True , 1:=True , 2:=True , 3:=True )) = True "
+lemma sc_threshold_2_3_tttt: 
+  "boolfunc_from_sc 4 sc_threshold_2_3 (a(0:=True,1:=True,2:=True,3:=True)) = True "
   unfolding hlp1 boolfunc_from_sc_def sc_threshold_2_3_def by auto
-
-(*lemma "bf_from_sc sc_threshold_2_3 = bool_fun_threshold_2_3"
-  unfolding sc_threshold_2_3_def
-  unfolding bool_fun_threshold_2_3_def
-  unfolding bf_from_sc_def
-  apply auto apply (rule ext)
-  unfolding count_true_def
-  using simplicial_complex.simplicial_complex_induced_by_monotone_boolean_function_4_bool_fun_threshold_2_3
-  using sc_threshold_2_3_ttft  
-  unfolding simplicial_complex_induced_by_monotone_boolean_function_def try
-  apply auto
-  apply (rule ext)
-  using card_boolean_function
-  try apply auto
-  oops (* nyeah, not gonna repeat that one *)
-*)
 
 lemma "boolfunc_from_sc n UNIV = bf_True"
   unfolding boolfunc_from_sc_def by simp
 
-text\<open>This may seem like an extra step, but effectively, it means: require that all the atoms outside the vertex are true, but don't care about what's in the vertex.\<close>
+lemma "boolfunc_from_sc n {} = bf_False"
+  unfolding boolfunc_from_sc_def by simp
+
+text\<open>This may seem like an extra step, but effectively, it means: 
+  require that all the atoms outside the vertex are true, 
+  but don't care about what's in the vertex.\<close>
 
 lemma boolfunc_from_sc_lazy: 
-  "simplicial_complex.simplicial_complex n K \<Longrightarrow> boolfunc_from_sc n K = (\<lambda>p. Pow {i. i < n \<and> \<not> p i} \<subseteq> K)"
+  "simplicial_complex.simplicial_complex n K 
+    \<Longrightarrow> boolfunc_from_sc n K = (\<lambda>p. Pow {i. i < n \<and> \<not> p i} \<subseteq> K)"
   unfolding simplicial_complex.simplicial_complex_def boolfunc_from_sc_def
   by auto (* wow *)
 
 primrec boolfunc_from_vertex_list :: "nat list \<Rightarrow> nat list \<Rightarrow> (nat \<Rightarrow> bool) \<Rightarrow> bool" 
   where
-  "boolfunc_from_vertex_list n [] = bf_True" |
-  "boolfunc_from_vertex_list n (f#fs) =  bf_and (boolfunc_from_vertex_list n fs) (if f \<in> set n then bf_True else bf_lit f)"
+  "boolfunc_from_vertex_list n [] = bf_True" | 
+  "boolfunc_from_vertex_list n (f#fs) =  
+      bf_and (boolfunc_from_vertex_list n fs) (if f \<in> set n then bf_True else bf_lit f)"
 
 lemma boolfunc_from_vertex_list_Cons: 
-  "boolfunc_from_vertex_list (a # as) lUNIV = (\<lambda>v. (boolfunc_from_vertex_list as lUNIV) (v(a:=True)))"
+  "boolfunc_from_vertex_list (a # as) lUNIV = 
+    (\<lambda>v. (boolfunc_from_vertex_list as lUNIV) (v(a:=True)))"
   by (induction lUNIV; simp add: bf_lit_def)
 
 lemma boolfunc_from_vertex_list_Empty: 
   "boolfunc_from_vertex_list [] lUNIV = Ball (set lUNIV)"
   by(induction lUNIV) (auto simp add: bf_lit_def)
 
-(*lemma "set lUNIV = UNIV \<Longrightarrow> boolfunc_from_vertex_list a lUNIV = (\<lambda>p. {i. \<not> p i} \<subseteq> set a)"
-  apply(induction "card (set lUNIV - set a)" arbitrary: a lUNIV)
-  oops*)
-  (* There is probably some neat way of proving this through an opposite-direction induction, but I'm not able to find an induction rule for it *)
-(* so I just prove it through straightforward induction and some helper lemmas *)
-
 lemma boolfunc_from_vertex_list:
   "set lUNIV = {..<n} \<Longrightarrow> boolfunc_from_vertex_list a lUNIV = (\<lambda>p. {i. i < n \<and> \<not> p i} \<subseteq> set a)"
-  by (induction a; fastforce simp add: boolfunc_from_vertex_list_Empty boolfunc_from_vertex_list_Cons)
-
-(*lemma boolfunc_from_vertex_list:
-  "set lUNIV = UNIV \<Longrightarrow> boolfunc_from_vertex_list a lUNIV = (\<lambda>p. {i. \<not> p i} \<subseteq> set a)"
-  by(induction a; fastforce simp add: boolfunc_from_vertex_list_Empty boolfunc_from_vertex_list_Cons)*)
+  by (induction a; fastforce 
+        simp add: boolfunc_from_vertex_list_Empty boolfunc_from_vertex_list_Cons)
 
 primrec boolfunc_from_sc_list :: "nat list \<Rightarrow> nat list list \<Rightarrow> (nat \<Rightarrow> bool) \<Rightarrow> bool" 
  where
    "boolfunc_from_sc_list lUNIV [] = bf_False" |
-   "boolfunc_from_sc_list lUNIV (l#L) = bf_or (boolfunc_from_sc_list lUNIV L) (boolfunc_from_vertex_list l lUNIV)"
+   "boolfunc_from_sc_list lUNIV (l#L) = 
+      bf_or (boolfunc_from_sc_list lUNIV L) (boolfunc_from_vertex_list l lUNIV)"
 
-lemma boolfunc_from_sc_un: "boolfunc_from_sc n (a\<union>b) = bf_or (boolfunc_from_sc n a) (boolfunc_from_sc n b)"
+lemma boolfunc_from_sc_un: 
+  "boolfunc_from_sc n (a\<union>b) = bf_or (boolfunc_from_sc n a) (boolfunc_from_sc n b)"
   unfolding boolfunc_from_sc_def unfolding bf_or_def bf_ite_def by force
 
 lemma bf_ite_const[simp]: "bf_ite bf_True a b = a" "bf_ite bf_False a b = b"
@@ -158,10 +164,13 @@ lemma bf_ite_const[simp]: "bf_ite bf_True a b = a" "bf_ite bf_False a b = b"
 lemma Pow_subset_Pow: "Pow a \<subseteq> Pow b = (a \<subseteq> b)"
   by blast
 
-lemma boolfunc_from_sc_list_concat: "boolfunc_from_sc_list lUNIV (a @ b) = bf_or (boolfunc_from_sc_list lUNIV a) (boolfunc_from_sc_list lUNIV b)"
+lemma boolfunc_from_sc_list_concat: 
+  "boolfunc_from_sc_list lUNIV (a @ b) = 
+      bf_or (boolfunc_from_sc_list lUNIV a) (boolfunc_from_sc_list lUNIV b)"
   by (induction a; auto)
 
-lemma boolfunc_from_sc_list_existing_useless: "a \<in> set as \<Longrightarrow> boolfunc_from_sc_list l (a # as) = boolfunc_from_sc_list l as"
+lemma boolfunc_from_sc_list_existing_useless: 
+  "a \<in> set as \<Longrightarrow> boolfunc_from_sc_list l (a # as) = boolfunc_from_sc_list l as"
 proof(induction as)
   case (Cons a1s as) then show ?case by (cases "a1s = a"; simp) metis
 qed simp
@@ -177,7 +186,8 @@ lemma set_remove[simp]: "set (remove a as) = set as - {a}"
 lemma remove_concat[simp]: "remove a (a1 @ a2) = remove a a1 @ remove a a2"
   by(induction a1; simp)
 
-lemma boolfunc_from_sc_list_dedup1: "boolfunc_from_sc_list l (a # as) = boolfunc_from_sc_list l (a # remove a as)"
+lemma boolfunc_from_sc_list_dedup1: 
+  "boolfunc_from_sc_list l (a # as) = boolfunc_from_sc_list l (a # remove a as)"
 proof(induction as)
   case (Cons a1s as) then show ?case by(cases "a1s = a"; simp) metis
 qed simp
@@ -189,7 +199,9 @@ next
   case (Cons a1 a2)
   then obtain b1 b2 where  b: "b = b1 @ a1 # b2" by (metis list.set_intros(1) split_list)
   have cons_concat: "\<And>a as. a # as = [a] @ as" by simp
-  have bb: "boolfunc_from_sc_list l b = bf_or (boolfunc_from_vertex_list a1 l) (bf_or (boolfunc_from_sc_list l b1) (boolfunc_from_sc_list l b2))"
+  have bb: "boolfunc_from_sc_list l b = 
+      bf_or (boolfunc_from_vertex_list a1 l) 
+            (bf_or (boolfunc_from_sc_list l b1) (boolfunc_from_sc_list l b2))"
     apply(subst b)
     apply(subst boolfunc_from_sc_list_concat)
     apply(subst cons_concat)
@@ -211,7 +223,9 @@ next
 qed simp
 
 lemma boolfunc_from_sc_list: 
-  "set lUNIV = {..<n::nat} \<Longrightarrow> simplicial_complex.simplicial_complex n (set ` set L) \<Longrightarrow> boolfunc_from_sc_list lUNIV L = boolfunc_from_sc n (set ` set L)"
+  "set lUNIV = {..<n::nat} 
+    \<Longrightarrow> simplicial_complex.simplicial_complex n (set ` set L) 
+      \<Longrightarrow> boolfunc_from_sc_list lUNIV L = boolfunc_from_sc n (set ` set L)"
 proof -
   assume lUNIV: "set lUNIV = {..<n::nat}"
   assume sc: "simplicial_complex.simplicial_complex n (set ` set L)"
@@ -261,27 +275,28 @@ qed
 
 lemma boolfunc_from_sc_alt: "boolfunc_from_sc n K = vec_to_boolfunc n (bf_from_sc K)"
   unfolding boolfunc_from_sc_def vec_to_boolfunc_def bf_from_sc_def
-  unfolding dim_vec apply auto apply (rule ext, safe)
+  unfolding dim_vec apply (rule ext, safe)
   by (smt (z3) Collect_cong index_vec)+
 
-text\<open>Another stone in the way: BDD assumes that the atoms are nats. So you'll need a function to map between @{typ "'a :: finite"} and @{typ "nat"}\<close>
-
-primrec bdd_from_vertex_list :: "nat list \<Rightarrow> nat list \<Rightarrow> bddi \<Rightarrow> (nat \<times> bddi) Heap" where
-"bdd_from_vertex_list n [] s = tci s" |
-"bdd_from_vertex_list n (f#fs) s = do {
-  (f, s) \<leftarrow> if f \<in> set n then tci s else litci f s;
-  (fs, s) \<leftarrow> bdd_from_vertex_list n fs s;
-  andci fs f s
+primrec bdd_from_vertex_list :: "nat list \<Rightarrow> nat list \<Rightarrow> bddi \<Rightarrow> (nat \<times> bddi) Heap" 
+  where
+    "bdd_from_vertex_list n [] s = tci s" |
+    "bdd_from_vertex_list n (f#fs) s = do {
+      (f, s) \<leftarrow> if f \<in> set n then tci s else litci f s;
+      (fs, s) \<leftarrow> bdd_from_vertex_list n fs s;
+    andci fs f s
 }"
+
 (* You'd guess that andci is commutative, and thus the argument order doesn't matter.
    You'd be wrong. The automation very much doesn't know about that. *)
 
-primrec bdd_from_sc_list :: "nat list \<Rightarrow> nat list list \<Rightarrow> bddi \<Rightarrow> (nat \<times> bddi) Heap" where
-"bdd_from_sc_list lUNIV [] s = fci s" |
-"bdd_from_sc_list lUNIV (l#L) s = do {
-  (l, s) \<leftarrow> bdd_from_vertex_list l lUNIV s;
-  (L, s) \<leftarrow> bdd_from_sc_list lUNIV L s;
-  orci L l s
+primrec bdd_from_sc_list :: "nat list \<Rightarrow> nat list list \<Rightarrow> bddi \<Rightarrow> (nat \<times> bddi) Heap" 
+  where
+    "bdd_from_sc_list lUNIV [] s = fci s" |
+    "bdd_from_sc_list lUNIV (l#L) s = do {
+      (l, s) \<leftarrow> bdd_from_vertex_list l lUNIV s;
+      (L, s) \<leftarrow> bdd_from_sc_list lUNIV L s;
+      orci L l s
 }"
 
 definition "nat_list_from_vertex v \<equiv> sorted_list_of_set (v)"
@@ -333,19 +348,31 @@ definition "ex_false \<equiv> do {
 
 definition "ex_true \<equiv> do {
   s \<leftarrow> emptyci;
-  (ex, s) \<leftarrow> bdd_from_sc_list [0, 1, 2, 3] (nat_list_from_sc {{},{0},{1},{2},{3},{0,1},{0,2},{0,3},{1,2},{1,3},{2,3},{0,1,2},{0,1,3},{0,2,3},{1,2,3},{0,1,2,3}}) s;
+  (ex, s) \<leftarrow> bdd_from_sc_list [0, 1, 2, 3] 
+      (nat_list_from_sc 
+      {{},{0},{1},{2},{3},
+       {0,1},{0,2},{0,3},{1,2},{1,3},{2,3},
+       {0,1,2},{0,1,3},{0,2,3},{1,2,3},{0,1,2,3}}) s;
   graphifyci ''true'' ex s
 }"
 
 definition "another_ex \<equiv> do {
   s \<leftarrow> emptyci;
-  (ex, s) \<leftarrow> bdd_from_sc_list [0, 1, 2, 3] (nat_list_from_sc {{},{0},{1},{2},{3},{0,1},{0,2},{0,3},{1,2},{1,3},{2,3},{0,1,2},{0,1,3},{0,2,3},{1,2,3}}) s;
+  (ex, s) \<leftarrow> bdd_from_sc_list [0, 1, 2, 3] 
+      (nat_list_from_sc 
+        {{},{0},{1},{2},{3},
+         {0,1},{0,2},{0,3},{1,2},{1,3},{2,3},
+         {0,1,2},{0,1,3},{0,2,3},{1,2,3}}) s;
   graphifyci ''another_ex'' ex s
 }"
 
 definition "one_another_ex \<equiv> do {
   s \<leftarrow> emptyci;
-  (ex, s) \<leftarrow> bdd_from_sc_list [0, 1, 2, 3] (nat_list_from_sc {{},{0},{1},{2},{3},{0,1},{0,2},{0,3},{1,2},{1,3},{2,3},{0,1,2},{0,1,3},{1,2,3}}) s;
+  (ex, s) \<leftarrow> bdd_from_sc_list [0, 1, 2, 3] 
+            (nat_list_from_sc 
+            {{},{0},{1},{2},{3},
+             {0,1},{0,2},{0,3},{1,2},{1,3},{2,3},
+             {0,1,2},{0,1,3},{1,2,3}}) s;
   graphifyci ''one_another_ex'' ex s
 }"
 
@@ -367,7 +394,8 @@ next
   show ?case proof(cases "a \<in> set n")
     case True
     show ?thesis
-      apply(simp only: bdd_from_vertex_list.simps list.map boolfunc_from_vertex_list.simps True if_True)
+      apply(simp only: bdd_from_vertex_list.simps list.map 
+          boolfunc_from_vertex_list.simps True if_True)
       apply(sep_auto simp only:)
        apply(rule Cons.IH)
       apply(clarsimp simp del: bf_ite_def)
@@ -376,7 +404,8 @@ next
   next
     case False
     show ?thesis
-      apply(simp only: bdd_from_vertex_list.simps list.map boolfunc_from_vertex_list.simps False if_False)
+      apply(simp only: bdd_from_vertex_list.simps list.map 
+          boolfunc_from_vertex_list.simps False if_False)
       apply(sep_auto simp only:)
        apply(rule Cons.IH)
       apply(sep_auto simp del: bf_ite_def bf_and_def)
@@ -399,7 +428,8 @@ qed
 lemma map_map_idI: "(\<And>x. x \<in> \<Union>(set ` set l) \<Longrightarrow> f x = x) \<Longrightarrow> map (map f) l = l"
   by(induct l; simp; meson map_idI)
 
-definition "bdd_from_sc K n \<equiv> bdd_from_sc_list (nat_list_from_vertex {..<n}) (nat_list_from_sc K)"
+definition 
+  "bdd_from_sc K n \<equiv> bdd_from_sc_list (nat_list_from_vertex {..<n}) (nat_list_from_sc K)"
 
 theorem bdd_from_sc:
   assumes "simplicial_complex.simplicial_complex n (K :: nat set set)"
