Binary_operations.thy
@@ -3,6 +3,10 @@ theory Binary_operations
  imports Bij_betw_simplicial_complex_bool_func
 begin
 
+text\<open>In this theory some results on binary operations over Boolean functions and
+  their relationship to operations over the induced simplicial complexes are
+  presented. We follow the presentation by Chastain and Scoville~\cite[Sect. 1.1]{CHSC}.\<close>
+
 definition bool_fun_or :: "nat \<Rightarrow> (bool vec \<Rightarrow> bool) \<Rightarrow> (bool vec \<Rightarrow> bool) \<Rightarrow> (bool vec \<Rightarrow> bool)"
   where "(bool_fun_or n f g) \<equiv> (\<lambda>x. f x \<or> g x)"
 
@@ -11,7 +15,8 @@ definition bool_fun_and :: "nat \<Rightarrow> (bool vec \<Rightarrow> bool) \<Ri
 
 lemma eq_union_or: 
   "simplicial_complex_induced_by_monotone_boolean_function n (bool_fun_or n f g)
-  = simplicial_complex_induced_by_monotone_boolean_function n f \<union> simplicial_complex_induced_by_monotone_boolean_function n g"
+  = simplicial_complex_induced_by_monotone_boolean_function n f 
+    \<union> simplicial_complex_induced_by_monotone_boolean_function n g"
   (is "?sc n (?bf_or n f g) = ?sc n f \<union> ?sc n g")
 proof
   show "?sc n f \<union> ?sc n g \<subseteq> ?sc n (?bf_or n f g)"
@@ -47,19 +52,23 @@ next
       unfolding simplicial_complex_induced_by_monotone_boolean_function_def
       unfolding ceros_of_boolean_input_def
       by auto (smt (verit) dim_vec eq_vecI index_vec)+
-    hence "(f (simplicial_complex.bool_vec_from_simplice n \<sigma>)) \<or> (g (simplicial_complex.bool_vec_from_simplice n \<sigma>))"
+    hence "(f (simplicial_complex.bool_vec_from_simplice n \<sigma>)) 
+            \<or> (g (simplicial_complex.bool_vec_from_simplice n \<sigma>))"
       unfolding bool_fun_or_def
       by auto
     hence "\<sigma> \<in> ?sc n f \<or> \<sigma> \<in> ?sc n g"
-      by (smt (z3) sigma bool_fun_or_def mem_Collect_eq simplicial_complex_induced_by_monotone_boolean_function_def)
-    thus "\<sigma> \<in> simplicial_complex_induced_by_monotone_boolean_function n f \<union> simplicial_complex_induced_by_monotone_boolean_function n g"
+      by (smt (z3) sigma bool_fun_or_def mem_Collect_eq 
+            simplicial_complex_induced_by_monotone_boolean_function_def)
+    thus "\<sigma> \<in> simplicial_complex_induced_by_monotone_boolean_function n f 
+          \<union> simplicial_complex_induced_by_monotone_boolean_function n g"
       by auto
   qed
 qed
 
 lemma eq_inter_and:
   "simplicial_complex_induced_by_monotone_boolean_function n (bool_fun_and n f g)
-  = simplicial_complex_induced_by_monotone_boolean_function n f \<inter> simplicial_complex_induced_by_monotone_boolean_function n g"
+  = simplicial_complex_induced_by_monotone_boolean_function n f 
+    \<inter> simplicial_complex_induced_by_monotone_boolean_function n g"
   (is "?sc n (?bf_and n f g) = ?sc n f \<inter> ?sc n g")
 proof
   show "?sc n f \<inter> ?sc n g \<subseteq> ?sc n (?bf_and n f g)"
@@ -96,34 +105,40 @@ next
       unfolding simplicial_complex_induced_by_monotone_boolean_function_def
       unfolding ceros_of_boolean_input_def
       by auto (smt (verit) dim_vec eq_vecI index_vec)+
-    hence "(f (simplicial_complex.bool_vec_from_simplice n \<sigma>)) \<and> (g (simplicial_complex.bool_vec_from_simplice n \<sigma>))"
+    hence "(f (simplicial_complex.bool_vec_from_simplice n \<sigma>)) 
+          \<and> (g (simplicial_complex.bool_vec_from_simplice n \<sigma>))"
       unfolding bool_fun_and_def
       by auto
     hence "\<sigma> \<in> ?sc n f \<and> \<sigma> \<in> ?sc n g"
       using bool_fun_and_def sigma simplicial_complex_induced_by_monotone_boolean_function_def by auto
-    thus "\<sigma> \<in> simplicial_complex_induced_by_monotone_boolean_function n f \<inter> simplicial_complex_induced_by_monotone_boolean_function n g"
+    thus "\<sigma> \<in> simplicial_complex_induced_by_monotone_boolean_function n f 
+          \<inter> simplicial_complex_induced_by_monotone_boolean_function n g"
       by auto
   qed
 qed
 
-definition bool_fun_ast :: "(nat \<times> nat) \<Rightarrow> (bool vec \<Rightarrow> bool) \<times> (bool vec \<Rightarrow> bool) \<Rightarrow> (bool vec \<times> bool vec \<Rightarrow> bool)"
+definition bool_fun_ast :: "(nat \<times> nat) \<Rightarrow> (bool vec \<Rightarrow> bool) \<times> (bool vec \<Rightarrow> bool) 
+    \<Rightarrow> (bool vec \<times> bool vec \<Rightarrow> bool)"
   where "(bool_fun_ast n f) \<equiv> (\<lambda> (x,y). (fst f x) \<and> (snd f y))"
 
 definition
   simplicial_complex_induced_by_monotone_boolean_function_ast
     :: "(nat \<times> nat) \<Rightarrow> ((bool vec \<times> bool vec \<Rightarrow> bool)) \<Rightarrow> (nat set * nat set) set"
   where "simplicial_complex_induced_by_monotone_boolean_function_ast n f =
-        {z. \<exists>x y. dim_vec x = fst n \<and> dim_vec y = snd n \<and> f (x, y) \<and> ((ceros_of_boolean_input x), (ceros_of_boolean_input y)) = z}"
+        {z. \<exists>x y. dim_vec x = fst n \<and> dim_vec y = snd n \<and> f (x, y) 
+          \<and> ((ceros_of_boolean_input x), (ceros_of_boolean_input y)) = z}"
 
 lemma fst_es_simplice:
   "a \<in> simplicial_complex_induced_by_monotone_boolean_function_ast n f
     \<Longrightarrow> (\<exists>x y. f (x, y) \<and> (ceros_of_boolean_input x) = fst(a))"
-  by (smt (verit) fst_conv mem_Collect_eq simplicial_complex_induced_by_monotone_boolean_function_ast_def)
+  by (smt (verit) fst_conv mem_Collect_eq 
+        simplicial_complex_induced_by_monotone_boolean_function_ast_def)
 
 lemma snd_es_simplice:
   "a \<in> simplicial_complex_induced_by_monotone_boolean_function_ast n f 
     \<Longrightarrow> (\<exists>x y. f (x, y) \<and> (ceros_of_boolean_input y) = snd(a))"
-  by (smt (verit) snd_conv mem_Collect_eq simplicial_complex_induced_by_monotone_boolean_function_ast_def)
+  by (smt (verit) snd_conv mem_Collect_eq 
+      simplicial_complex_induced_by_monotone_boolean_function_ast_def)
 
 definition set_ast :: "(nat set) set \<Rightarrow> (nat set) set \<Rightarrow> ((nat set*nat set) set)"
   where "set_ast A B \<equiv> {c. \<exists>a\<in>A. \<exists>b\<in>B. c = (a,b)}"
@@ -174,11 +189,13 @@ lemma
   unfolding simplicial_complex_induced_by_monotone_boolean_function_ast_def
   unfolding bool_fun_ast_def
   unfolding ceros_of_boolean_input_def
-  by auto (smt (verit, ccfv_threshold) bool_fun_ast_def case_prod_conv dim_vec index_vec vec_eq_iff)
+  by auto (smt (verit, ccfv_threshold) bool_fun_ast_def 
+        case_prod_conv dim_vec index_vec vec_eq_iff)
 
 lemma eq_ast:
 "simplicial_complex_induced_by_monotone_boolean_function_ast (n, m) (bool_fun_ast (n, m) f)
-= set_ast (simplicial_complex_induced_by_monotone_boolean_function n (fst f)) (simplicial_complex_induced_by_monotone_boolean_function m (snd f))"
+= set_ast (simplicial_complex_induced_by_monotone_boolean_function n (fst f)) 
+          (simplicial_complex_induced_by_monotone_boolean_function m (snd f))"
 proof
   show "set_ast (simplicial_complex_induced_by_monotone_boolean_function n (fst f))
      (simplicial_complex_induced_by_monotone_boolean_function m (snd f))
@@ -197,10 +214,14 @@ proof
       unfolding set_ast_def by auto
     have tau: "(snd f) (simplicial_complex.bool_vec_from_simplice m (snd \<gamma>))"
       using simplicial_complex.simplicial_complex_implies_true [OF g] .
-    from sigma and tau have sigtau: "bool_fun_ast (n, m) f ((simplicial_complex.bool_vec_from_simplice n (fst \<gamma>)), (simplicial_complex.bool_vec_from_simplice m (snd \<gamma>)))"
+    from sigma and tau have sigtau: "bool_fun_ast (n, m) f 
+        ((simplicial_complex.bool_vec_from_simplice n (fst \<gamma>)), 
+         (simplicial_complex.bool_vec_from_simplice m (snd \<gamma>)))"
       unfolding bool_fun_ast_def
       by auto
-    from sigtau show "\<gamma> \<in> simplicial_complex_induced_by_monotone_boolean_function_ast (n, m) (bool_fun_ast (n, m) f)"
+    from sigtau 
+    show "\<gamma> \<in> simplicial_complex_induced_by_monotone_boolean_function_ast (n, m) 
+              (bool_fun_ast (n, m) f)"
       unfolding simplicial_complex_induced_by_monotone_boolean_function_ast_def
       unfolding bool_fun_ast_def
       using sigma apply auto
@@ -212,7 +233,7 @@ next
     \<subseteq> set_ast (simplicial_complex_induced_by_monotone_boolean_function n (fst f))
         (simplicial_complex_induced_by_monotone_boolean_function m (snd f))"
     proof
-    fix \<gamma>::"nat set*nat set"
+    fix \<gamma> :: "nat set*nat set"
     assume pert: "\<gamma> \<in> simplicial_complex_induced_by_monotone_boolean_function_ast (n, m)
      (bool_fun_ast (n, m) f)"
     have sigma: "(fst \<gamma>) \<in> simplicial_complex_induced_by_monotone_boolean_function n (fst f)"
@@ -223,8 +244,11 @@ next
       apply (rule exI [of _ "simplicial_complex.bool_vec_from_simplice n (fst \<gamma>)"], safe)
       using simplicial_complex.bool_vec_from_simplice_def apply auto[1]
         apply (metis fst_conv pert simplicial_complex_ast_implies_fst_true)
-      using ceros_of_boolean_input_def simplicial_complex.bool_vec_from_simplice_def apply fastforce
-      using ceros_of_boolean_input_def pert simplicial_complex.bool_vec_from_simplice_def simplicial_complex_induced_by_monotone_boolean_function_ast_def by force
+      using ceros_of_boolean_input_def simplicial_complex.bool_vec_from_simplice_def 
+        apply fastforce
+      using ceros_of_boolean_input_def pert 
+          simplicial_complex.bool_vec_from_simplice_def 
+          simplicial_complex_induced_by_monotone_boolean_function_ast_def by force
    have tau: "(snd \<gamma>) \<in> simplicial_complex_induced_by_monotone_boolean_function m (snd f)"
       unfolding bool_fun_ast_def
       unfolding simplicial_complex_induced_by_monotone_boolean_function_def
@@ -233,9 +257,15 @@ next
       apply (rule exI [of _ "simplicial_complex.bool_vec_from_simplice m (snd \<gamma>)"], safe)
       using simplicial_complex.bool_vec_from_simplice_def apply auto[1]
         apply (metis snd_conv pert simplicial_complex_ast_implies_snd_true)
-      using ceros_of_boolean_input_def simplicial_complex.bool_vec_from_simplice_def apply fastforce
-      using ceros_of_boolean_input_def pert simplicial_complex.bool_vec_from_simplice_def simplicial_complex_induced_by_monotone_boolean_function_ast_def by force
-    from sigma and tau show "\<gamma> \<in> set_ast (simplicial_complex_induced_by_monotone_boolean_function n (fst f)) (simplicial_complex_induced_by_monotone_boolean_function m (snd f))"
+      using ceros_of_boolean_input_def simplicial_complex.bool_vec_from_simplice_def 
+       apply fastforce
+      using ceros_of_boolean_input_def pert 
+        simplicial_complex.bool_vec_from_simplice_def 
+        simplicial_complex_induced_by_monotone_boolean_function_ast_def by force
+    from sigma and tau 
+    show "\<gamma> \<in> set_ast 
+        (simplicial_complex_induced_by_monotone_boolean_function n (fst f)) 
+        (simplicial_complex_induced_by_monotone_boolean_function m (snd f))"
       using set_ast_def
       by force
   qed
